We want to show the equivalence of
\begin{center}
	$p(\tilde{f_i}|f_i) = \mathcal{N}(\tilde{f_i}|f_i, \sigma^2)$ with $p(y_i=1|\tilde{f_i}) =$ 
	\begin{cases}
		1,  & \text{if}\ \tilde{f_i}\geq 0 \\
      	0,  & \text{otherwise}
	\end{cases} 
\end{center}
\newline
and
\newline
\begin{center}
	$p(y_i=1|f_i) = \sigma_{probit}(f_i) = \frac{1}{\sqrt{2\pi}} \int_{-\infty}^{f_i} exp(-\frac{t^2}{2})dt$.
\end{center}
Therefore we integrate:
\begin{align*}
	\int_{-\infty}^\infty p(\tilde{f_i}|f_i) p(y_i=1|\tilde{f_i}) d\tilde{f_i} 
	=\int_{-\infty}^\infty \frac{1}{\sigma\sqrt{2\pi}} exp(-\frac{(\tilde{f_i}-f_i)^2}{2\sigma^2}) p(y_i|\tilde{f_i}) d\tilde{f_i} \\
\end{align*}
Because of the definition of $p(y_i|\tilde{f_i})$ we can rewrite:
\begin{align*}
	\int_{-\infty}^\infty p(\tilde{f_i}|f_i) p(y_i=1|\tilde{f_i}) d\tilde{f_i} 
	&=\int_0^\infty \frac{1}{\sigma\sqrt{2\pi}} exp(-\frac{(\tilde{f_i}-f_i)^2}{2\sigma^2}) d\tilde{f_i} \\
	&=\int_0^{f_i} \frac{1}{\sigma\sqrt{2\pi}} exp(-\frac{t^2}{2\sigma^2}) dt \\
\end{align*}
Thus we have 
\begin{align*}
	\int_{-\infty}^\infty p(\tilde{f_i}|f_i) p(y_i=1|\tilde{f_i}) d\tilde{f_i}  
	=\frac{1}{\sigma\sqrt{2\pi}} \int_0^{f_i} exp(-\frac{t^2}{2\sigma^2}) dt
\end{align*}
and to match the function exactly we choose $\sigma^2=1$:
\begin{align*}
\frac{1}{1\sqrt{2\pi}} \int_0^{f_i} exp(-\frac{t^2}{2\cdot 1^2}) dt 
= \frac{1}{\sqrt{2\pi}} \int_0^{f_i} exp(-\frac{t^2}{2}) dt
\end{align*}

